@prefix :        <http://www.juntadeandalucia.es/servicioandaluzdesalud/ict/operational#> .
@prefix sas-ict: <http://www.juntadeandalucia.es/servicioandaluzdesalud/ict#> .
@prefix dcterms: <http://purl.org/dc/terms/> .
@prefix foaf:    <http://xmlns.com/foaf/0.1/> .
@prefix gr:      <http://purl.org/goodrelations/v1#> .
@prefix owl:     <http://www.w3.org/2002/07/owl#> .
@prefix qudt:    <http://qudt.org/schema/qudt#> .
@prefix rdf:     <http://www.w3.org/1999/02/22-rdf-syntax-ns#> .
@prefix rdfs:    <http://www.w3.org/2000/01/rdf-schema#> .
@prefix skos:    <http://www.w3.org/2004/02/skos/core#> .
@prefix spin:    <http://spinrdf.org/spin#> .
@prefix time:    <http://www.w3.org/2006/time#> .
@prefix usdl-agreement:  <http://www.linked-usdl.org/ns/usdl-agreement#> .
@prefix usdl-br:  <http://www.linked-usdl.org/ns/usdl-business-roles#> .
@prefix usdl-core:  <http://www.linked-usdl.org/ns/usdl-core#> .
@prefix usdl-lr:  <http://www.linked-usdl.org/ns/usdl-liability-roles#> .
@prefix vcard:   <http://www.w3.org/2006/vcard/ns#> .
@prefix xsd:     <http://www.w3.org/2001/XMLSchema#> .

<http://www.juntadeandalucia.es/servicioandaluzdesalud/ict/operational>
      rdf:type owl:Ontology ;
      rdfs:label "SAS ICT operational services SLA ontology"@en ;
      rdfs:seeAlso <http://aws.amazon.com/ec2/sla/> ;
      dcterms:created "2015-11-15"^^xsd:date ;
      dcterms:description "This vocabulary has been created as part of the use case validation of Linked USDL Agreement module. It describes the service level agreement of the operational services described in a call for tenders published by the Andalusian Health Service (SAS), a regional public health care institution in Spain."@en ;
      dcterms:modified "2015-11-20"^^xsd:date, "2015-11-22"^^xsd:date ;
      dcterms:title "SAS ICT operational services SLA ontology"@en ;
      owl:imports <http://www.juntadeandalucia.es/servicioandaluzdesalud/ict> ;
      owl:versionInfo "1.0" .

#################################################
# BusinessEntity description for SAS ICT services

:andalusianHealthService
      rdf:type gr:BusinessEntity ;
      vcard:hasAddress
              [ rdf:type vcard:Work ;
                vcard:country-name "Spain"@en
              ] ;
      foaf:homepage <http://www.juntadeandalucia.es/servicioandaluzdesalud> ;
      foaf:logo <http://www.juntadeandalucia.es/servicioandaluzdesalud/images/juntalink.png> ;
      foaf:name "Servicio Andaluz de Salud"@es .

:tender
      rdf:type gr:BusinessEntity ;
      foaf:name "SAS ICT maintenance service tender" .

:tenderInvolvement
      rdf:type usdl-core:EntityInvolvement ;
      usdl-core:ofBusinessEntity :tender ;
      usdl-core:withBusinessRole usdl-agreement:metricProvider , usdl-br:provider .

:andalusianHealthServiceInvolvement
      rdf:type usdl-core:EntityInvolvement ;
	  usdl-core:ofBusinessEntity :andalusianHealthService ;
      usdl-core:withBusinessRole usdl-agreement:conditionEvaluator , usdl-br:customer .

:tenderLiability
      rdf:type usdl-agreement:EntityLiability ;
      usdl-core:ofBusinessEntity :tender ;
      usdl-core:withBusinessRole usdl-br:provider ;
      usdl-agreement:withLiabilityRole usdl-lr:guarantor .

:andalusianHealthServiceLiability
      rdf:type usdl-agreement:EntityLiability ;
      usdl-core:ofBusinessEntity :andalusianHealthService ;
      usdl-core:withBusinessRole usdl-br:customer ;
      usdl-agreement:withLiabilityRole usdl-lr:beneficiary .

:tenderLiabilityForMaximumPenaltyCosts
      rdf:type usdl-agreement:EntityLiability ;
      usdl-core:ofBusinessEntity :tender ;
      usdl-core:withBusinessRole usdl-br:provider ;
      usdl-agreement:withLiabilityRole usdl-lr:beneficiary .

:andalusianHealthServiceLiabilityForMaximumPenaltyCosts
      rdf:type usdl-agreement:EntityLiability ;
      usdl-core:ofBusinessEntity :andalusianHealthService ;
      usdl-core:withBusinessRole usdl-br:customer ;
      usdl-agreement:withLiabilityRole usdl-lr:guarantor .

      
############################################
# Individual services provided by the tender

:tenderIssueResolutionService
      rdf:type sas-ict:IssueResolutionService;
      rdfs:label "Tender Issue Resolution Service"^^xsd:string ;
      usdl-core:hasEntityInvolvement :tenderInvolvement .

:tenderDataRequestResolutionService
      rdf:type sas-ict:DataRequestResolutionService;
      rdfs:label "Tender Data Request Resolution Service"^^xsd:string ;
      usdl-core:hasEntityInvolvement :tenderInvolvement .

:tenderMiscellaneousRequestsResolutionService
      rdf:type sas-ict:MiscellaneousRequestsResolutionService;
      rdfs:label "Tender Miscellaneous Requests Resolution Service"^^xsd:string ;
      usdl-core:hasEntityInvolvement :tenderInvolvement .

########################################			  
# Service properties relevant to the SLA

:IO_01
      rdf:type owl:ObjectProperty ;
      rdfs:comment "Percentage of very high priority issues resolved in time."@en ;
      rdfs:subPropertyOf gr:quantitativeProductOrServiceProperty ;
      usdl-agreement:hasMetric :veryHighPriorityIssuesResolvedInTimePercentage .

:veryHighPriorityIssuesResolvedInTimePercentage
      rdf:type usdl-agreement:Metric ;
      qudt:unit <http://qudt.org/vocab/unit#Percent> ;
      rdfs:comment "Computation of percentage of very high priority issues resolved in time."@en ;
      usdl-agreement:hasExpression
              """SELECT  ?service (( ?timelyIssues / ?totalIssues ) AS ?IO_01)
                   WHERE
                     { ?service sas-ict:hasIssue ?issue
                         { SELECT  ?service (COUNT(?issue) AS ?totalIssues)
                           WHERE
                             { ?service sas-ict:hasIssue ?issue .
                               ?issue sas-ict:hasPriority sas-ict:VeryHighPriority
                             }
                           GROUP BY ?service
                         }
                       UNION
                         { SELECT  ?service (COUNT(?issue) AS ?timelyIssues)
                           WHERE
                             { ?service sas-ict:hasIssue ?issue .
                               ?issue sas-ict:hasPriority sas-ict:VeryHighPriority .
                               ?issue sas-ict:hasResolutionTime ?resTime .
                               ?resTime time:hasDurationDescription ?resDuration .
                               ?resDuration time:hours ?resDurationInHours
                               FILTER ( ?resDurationInHours < 2 )
                             }
                           GROUP BY ?service
                         }
                     }"""^^xsd:string ;
      usdl-agreement:hasMeasuringInterval :billingInterval .

:IO_04
      rdf:type owl:ObjectProperty ;
      rdfs:comment "Average resolution time of very high priority issues."@en ;
      rdfs:subPropertyOf gr:quantitativeProductOrServiceProperty ;
      usdl-agreement:hasMetric :veryHighPriorityIssuesAvgResolutionTime .

:veryHighPriorityIssuesAvgResolutionTime
      rdf:type usdl-agreement:Metric ;
      qudt:unit <http://qudt.org/vocab/unit#Hour> ;
      rdfs:comment "Computation of average resolution time of very high priority issues."@en ;
      usdl-agreement:hasExpression
              """SELECT  ?service (AVG(?resDurationInHours) AS ?IO_04)
                   WHERE
                     { ?service sas-ict:hasIssue ?issue .
                       ?issue sas-ict:hasPriority sas-ict:VeryHighPriority .
                       ?issue sas-ict:hasResolutionTime ?resTime .
                       ?resTime time:hasDurationDescription ?resDuration .
                       ?resDuration time:hours ?resDurationInHours
                     }
                   GROUP BY ?service"""^^xsd:string ;
      usdl-agreement:hasMeasuringInterval :billingInterval .

:IO_05
      rdf:type owl:ObjectProperty ;
      rdfs:comment "Average resolution time of high priority issues."@en ;
      rdfs:subPropertyOf gr:quantitativeProductOrServiceProperty ;
      usdl-agreement:hasMetric :highPriorityIssuesAvgResolutionTime .

:highPriorityIssuesAvgResolutionTime
      rdf:type usdl-agreement:Metric ;
      qudt:unit <http://qudt.org/vocab/unit#Hour> ;
      rdfs:comment "Computation of average resolution time of high priority issues."@en ;
      usdl-agreement:hasExpression
              """SELECT  ?service (AVG(?resDurationInHours) AS ?IO_05)
                   WHERE
                     { ?service sas-ict:hasIssue ?issue .
                       ?issue sas-ict:hasPriority sas-ict:HighPriority .
                       ?issue sas-ict:hasResolutionTime ?resTime .
                       ?resTime time:hasDurationDescription ?resDuration .
                       ?resDuration time:hours ?resDurationInHours
                     }
                   GROUP BY ?service"""^^xsd:string ;
      usdl-agreement:hasMeasuringInterval :billingInterval .

:billingInterval
      rdf:type time:Interval ;
      time:hasDurationDescription
              [ rdf:type time:DurationDescription ;
                time:months 1 
              ] .
              
:contractInterval
      rdf:type time:Interval ;
      time:hasDurationDescription
              [ rdf:type time:DurationDescription ;
                time:years 2 
              ] .

:slaExclusionInterval
      rdf:type time:Interval ;
      time:intervalStartedBy :contractInterval ;
      time:intervalBefore :slaValidityInterval ;
      time:hasDurationDescription
              [ rdf:type time:DurationDescription ;
                time:weeks 8
              ] .
 
:slaValidityInterval
      rdf:type time:Interval ;
      time:hasDurationDescription
              [ rdf:type time:DurationDescription ;
                time:years 1 ;
                time:weeks 44
              ] .

:IO_01PenaltyCost
      rdf:type owl:ObjectProperty ;
      rdfs:comment "Percentage with respect to monthly incurred costs to be deducted when IO_01 commitment is not enforced."@en ;
      rdfs:subPropertyOf sas-ict:timeBoundedQuantitativeProductOrServiceProperty .

:IO_02PenaltyCost
      rdf:type owl:ObjectProperty ;
      rdfs:comment "Percentage with respect to monthly incurred costs to be deducted when IO_02 commitment is not enforced."@en ;
      rdfs:subPropertyOf sas-ict:timeBoundedQuantitativeProductOrServiceProperty .

:IO_03PenaltyCost
      rdf:type owl:ObjectProperty ;
      rdfs:comment "Percentage with respect to monthly incurred costs to be deducted when IO_03 commitment is not enforced."@en ;
      rdfs:subPropertyOf sas-ict:timeBoundedQuantitativeProductOrServiceProperty .

:IO_04PenaltyCost
      rdf:type owl:ObjectProperty ;
      rdfs:comment "Percentage with respect to monthly incurred costs to be deducted when IO_04 commitment is not enforced."@en ;
      rdfs:subPropertyOf sas-ict:timeBoundedQuantitativeProductOrServiceProperty .

:IO_05PenaltyCost
      rdf:type owl:ObjectProperty ;
      rdfs:comment "Percentage with respect to monthly incurred costs to be deducted when IO_05 commitment is not enforced."@en ;
      rdfs:subPropertyOf sas-ict:timeBoundedQuantitativeProductOrServiceProperty .

:IO_06PenaltyCost
      rdf:type owl:ObjectProperty ;
      rdfs:comment "Percentage with respect to monthly incurred costs to be deducted when IO_06 commitment is not enforced."@en ;
      rdfs:subPropertyOf sas-ict:timeBoundedQuantitativeProductOrServiceProperty .

:IO_07PenaltyCost
      rdf:type owl:ObjectProperty ;
      rdfs:comment "Percentage with respect to monthly incurred costs to be deducted when IO_07 commitment is not enforced."@en ;
      rdfs:subPropertyOf sas-ict:timeBoundedQuantitativeProductOrServiceProperty .

:IO_08PenaltyCost
      rdf:type owl:ObjectProperty ;
      rdfs:comment "Percentage with respect to monthly incurred costs to be deducted when IO_08 commitment is not enforced."@en ;
      rdfs:subPropertyOf sas-ict:timeBoundedQuantitativeProductOrServiceProperty .

:IO_09PenaltyCost
      rdf:type owl:ObjectProperty ;
      rdfs:comment "Percentage with respect to monthly incurred costs to be deducted when IO_09 commitment is not enforced."@en ;
      rdfs:subPropertyOf sas-ict:timeBoundedQuantitativeProductOrServiceProperty .

:IO_10PenaltyCost
      rdf:type owl:ObjectProperty ;
      rdfs:comment "Percentage with respect to monthly incurred costs to be deducted when IO_10 commitment is not enforced."@en ;
      rdfs:subPropertyOf sas-ict:timeBoundedQuantitativeProductOrServiceProperty .

:IO_11PenaltyCost
      rdf:type owl:ObjectProperty ;
      rdfs:comment "Percentage with respect to monthly incurred costs to be deducted when IO_11 commitment is not enforced."@en ;
      rdfs:subPropertyOf sas-ict:timeBoundedQuantitativeProductOrServiceProperty .

:IO_12PenaltyCost
      rdf:type owl:ObjectProperty ;
      rdfs:comment "Percentage with respect to monthly incurred costs to be deducted when IO_12 commitment is not enforced."@en ;
      rdfs:subPropertyOf sas-ict:timeBoundedQuantitativeProductOrServiceProperty .

:IO_13PenaltyCost
      rdf:type owl:ObjectProperty ;
      rdfs:comment "Percentage with respect to monthly incurred costs to be deducted when IO_13 commitment is not enforced."@en ;
      rdfs:subPropertyOf sas-ict:timeBoundedQuantitativeProductOrServiceProperty .

:IO_14PenaltyCost
      rdf:type owl:ObjectProperty ;
      rdfs:comment "Percentage with respect to monthly incurred costs to be deducted when IO_14 commitment is not enforced."@en ;
      rdfs:subPropertyOf sas-ict:timeBoundedQuantitativeProductOrServiceProperty .

:IO_15PenaltyCost
      rdf:type owl:ObjectProperty ;
      rdfs:comment "Percentage with respect to monthly incurred costs to be deducted when IO_15 commitment is not enforced."@en ;
      rdfs:subPropertyOf sas-ict:timeBoundedQuantitativeProductOrServiceProperty .

:monthlyPenaltyCost
      rdf:type owl:ObjectProperty ;
      rdfs:comment "Percentage with respect to monthly incurred costs to be deducted each month."@en ;
      rdfs:subPropertyOf sas-ict:timeBoundedQuantitativeProductOrServiceProperty ;
      usdl-agreement:hasMetric :monthlyPenaltyCostMetric .

:monthlyPenaltyCostMetric
      rdf:type usdl-agreement:Metric ;
      qudt:unit <http://qudt.org/vocab/unit#Percent> ;
      rdfs:comment "Metric to compute the percentage with respect to monthly incurred costs to be deducted each month."@en ;
      usdl-agreement:hasExpression
              """SELECT ?service ?billingInterval (SUM(?penaltyCost) AS ?monthlyPenaltyCost)
                   WHERE
                     { ?service rdf:type sas-ict:OperationalServices .
                       VALUES ?penaltyCostProperty { :IO_01PenaltyCost :IO_02PenaltyCost :IO_03PenaltyCost :IO_04PenaltyCost :IO_05PenaltyCost :IO_06PenaltyCost :IO_07PenaltyCost :IO_08PenaltyCost :IO_09PenaltyCost :IO_10PenaltyCost :IO_11PenaltyCost :IO_12PenaltyCost :IO_13PenaltyCost :IO_14PenaltyCost :IO_15PenaltyCost }
                       ?service ?penaltyCostProperty ?penaltyCost .
                       ?penaltyCost sas-ict:spansInterval ?billingInterval
                     }
                   GROUP BY ?service ?billingInterval"""^^xsd:string ;
      usdl-agreement:hasMeasuringInterval :billingInterval .

:totalPenaltyCost
      rdf:type owl:ObjectProperty ;
      rdfs:comment "Percentage with respect to the total incurred costs during the whole contract that has been deducted."@en ;
      rdfs:subPropertyOf gr:quantitativeProductOrServiceProperty ;
      usdl-agreement:hasMetric :totalPenaltyCostMetric .

:totalPenaltyCostMetric
      rdf:type usdl-agreement:Metric ;
      qudt:unit <http://qudt.org/vocab/unit#Percent> ;
      rdfs:comment "Metric to compute the percentage with respect to the total incurred costs during the whole contract to be deducted."@en ;
      usdl-agreement:hasExpression
              """SELECT ?service (SUM(?penaltyCost * ?incurredCost) AS ?totalPenaltyCost)
                   WHERE
                     { ?service rdf:type sas-ict:OperationalServices .
                       VALUES ?penaltyCostProperty { :IO_01PenaltyCost :IO_02PenaltyCost :IO_03PenaltyCost :IO_04PenaltyCost :IO_05PenaltyCost :IO_06PenaltyCost :IO_07PenaltyCost :IO_08PenaltyCost :IO_09PenaltyCost :IO_10PenaltyCost :IO_11PenaltyCost :IO_12PenaltyCost :IO_13PenaltyCost :IO_14PenaltyCost :IO_15PenaltyCost }
                       ?service ?penaltyCostProperty ?penaltyCost .
                       ?penaltyCost sas-ict:spansInterval ?billingInterval .
                       ?service sas-ict:incurredCost ?incurredCost .
                       ?incurredCost sas-ict:spansInterval ?billingInterval
                     }
                   GROUP BY ?service"""^^xsd:string ;
      usdl-agreement:hasMeasuringInterval :billingInterval .

#######################################
# Sample service offering including SLA

:operationalServiceOffering
      rdf:type usdl-core:ServiceOffering ;
      usdl-agreement:hasAgreementTerm :IO_01Commitment , :IO_04Commitment ; # tender commitments
      usdl-agreement:hasAgreementTerm :monthlyPenaltyCostCommitment , :totalPenaltyCostCommitment ; # SAS commitments
      usdl-core:hasEntityInvolvement :andalusianHealthServiceInvolvement , :tenderInvolvement ;
      usdl-core:includes :tenderIssueResolutionService, :tenderDataRequestResolutionService, :tenderMiscellaneousRequestsResolutionService .

:IO_04Commitment
      rdf:type usdl-agreement:Guarantee ;
      usdl-agreement:guaranteedOver :tenderIssueResolutionService ;
      usdl-agreement:guarantees
              [ rdf:type usdl-agreement:MaxGuaranteedValue ;
                qudt:unit <http://qudt.org/vocab/unit#Hour> ;
				usdl-agreement:hasEvaluationInterval :billingInterval ;
                usdl-agreement:hasValue
                        [ rdf:type gr:QuantitativeValueFloat ;
                          gr:hasValueFloat "2"^^xsd:float
                        ] ;
                usdl-agreement:refersTo
                        :IO_04
              ] ;
      usdl-agreement:hasCompensation
              :IO_04Compensation ;
      usdl-agreement:hasEntityLiability :andalusianHealthServiceLiability , :tenderLiability ;
	  usdl-agreement:hasValidityInterval :slaValidityInterval .
	  
################################################################################
# Limitations to penalty costs guaranteed by the Andalusian Health Service (SAS)

:monthlyPenaltyCostCommitment
      rdf:type usdl-agreement:Guarantee ;
      usdl-agreement:guaranteedOver :tenderIssueResolutionService , :tenderDataRequestsResolutionService , :tenderMiscellaneousRequestsResolutionService ;
      usdl-agreement:guarantees
              [ rdf:type usdl-agreement:MaxGuaranteedValue ;
                qudt:unit <http://qudt.org/vocab/unit#Percent> ;
				usdl-agreement:hasEvaluationInterval :billingInterval ;
                usdl-agreement:hasValue
                        [ rdf:type gr:QuantitativeValueFloat ;
                          gr:hasValueFloat "25"^^xsd:float
                        ] ;
                usdl-agreement:refersTo
                        :monthlyPenaltyCost
              ] ;
      usdl-agreement:hasEntityLiability :andalusianHealthServiceLiabilityForMaximumPenaltyCosts , :tenderLiabilityForMaximumPenaltyCosts ;
	  usdl-agreement:hasValidityInterval :contractInterval .

:totalPenaltyCostCommitment
      rdf:type usdl-agreement:Guarantee ;
      usdl-agreement:guaranteedOver :tenderIssueResolutionService , :tenderDataRequestsResolutionService , :tenderMiscellaneousRequestsResolutionService ;
      usdl-agreement:guarantees
              [ rdf:type usdl-agreement:MaxGuaranteedValue ;
                qudt:unit <http://qudt.org/vocab/unit#Percent> ;
				usdl-agreement:hasEvaluationInterval :contractInterval ;
                usdl-agreement:hasValue
                        [ rdf:type usdl-agreement:Metric ;
                          usdl-agreement:hasExpression "10% * ?totalBudget"^^xsd:string
                        ] ;
                usdl-agreement:refersTo
                        :totalPenaltyCost
              ] ;
      usdl-agreement:hasEntityLiability :andalusianHealthServiceLiabilityForMaximumPenaltyCosts , :tenderLiabilityForMaximumPenaltyCosts ;
	  usdl-agreement:hasValidityInterval :contractInterval .


###############
# Compensations

:IO_04Compensation
      rdf:type usdl-agreement:Compensation ;
      usdl-agreement:guarantees
              [ rdf:type usdl-agreement:GuaranteedValue ;
                qudt:unit <http://qudt.org/vocab/unit#Percent> ;
                usdl-agreement:hasValue
                        [ rdf:type usdl-agreement:Metric ;
                          usdl-agreement:hasExpression "(?IO_04 - 2) / 0,33) * 30% * 25%"^^xsd:string
                        ] ;
                usdl-agreement:refersTo
                        :IO_04PenaltyCost
              ] ;
      usdl-agreement:hasEntityLiability
              :andalusianHealthServiceLiability , :tenderLiability .
